Impl/MarshallingModel.i.dfy
@@ -55,24 +55,7 @@ module MarshallingModel {
 
   /////// Some lemmas that are useful in Impl
 
-  lemma WeightBucketLteSize(v: V, pivotTable: seq<Key>, i: int, kvl: KVList.Kvl)
-  requires Marshalling.valToBucket.requires(v)
-  requires KVList.WF(kvl)
-  requires Marshalling.valToBucket(v) == Some(KVList.I(kvl))
-  ensures WeightBucket(KVList.I(kvl)) <= SizeOfV(v)
-  {
-    /*KVList.kvlWeightEq(kvl);
-    reveal_SeqSum();
-    assert SizeOfV(v)
-        == SeqSum(v.t)
-        == SizeOfV(v.t[0]) + SeqSum(v.t[1..])
-        == SizeOfV(v.t[0]) + SizeOfV(v.t[1]) + SeqSum([])
-        == SizeOfV(v.t[0]) + SizeOfV(v.t[1])
-        == 8 + WeightKeySeq(v.t[0].ka) + 8 + WeightMessageSeq(v.t[1].ma);*/
-    assume false;
-  }
-
-  lemma WeightBucketListLteSize(v: V, pivotTable: seq<Key>, buckets: seq<Bucket>)
+  lemma WeightBucketListLteSize(v: V, buckets: seq<Bucket>)
   requires v.VArray?
   requires Marshalling.valToBuckets.requires(v.a)
   requires Marshalling.valToBuckets(v.a) == Some(buckets)
@@ -80,24 +63,25 @@ module MarshallingModel {
 
   decreases |v.a|
   {
-    /*reveal_WeightBucketList();
-    if |v.a| == 0 {
+    if |buckets| == 0 {
+      reveal_WeightBucketList();
     } else {
-      WeightBucketListLteSize(VArray(DropLast(v.a)), pivotTable, DropLast(buckets));
-      lemma_SeqSum_prefix(DropLast(v.a), Last(v.a));
+      var prebuckets := DropLast(buckets);
+      var prev := VArray(DropLast(v.a));
+      var lastbucket := Last(buckets);
+      var lastv := Last(v.a);
 
-      var pref := Marshalling.valToBuckets(DropLast(v.a), pivotTable).value;
-      var kvl := Marshalling.valToBucket(Last(v.a), pivotTable, |pref|).value;
-      WeightBucketLteSize(Last(v.a), pivotTable, |pref|, kvl);
-
-      assert DropLast(v.a) + [Last(v.a)] == v.a;
-      assert WeightBucketList(buckets)
-          == WeightBucketList(DropLast(buckets)) + WeightBucket(Last(buckets))
-          <= SizeOfV(VArray(DropLast(v.a))) + WeightBucket(Last(buckets))
-          <= SizeOfV(VArray(DropLast(v.a))) + SizeOfV(Last(v.a))
-          == SizeOfV(v);
-    }*/
-    assume false;
+      assume false; 
+      calc <= {
+        WeightBucketList(buckets);
+        { reveal_WeightBucketList(); }
+        WeightBucketList(prebuckets) + WeightBucket(lastbucket);
+        { WeightBucketListLteSize(prev, prebuckets); }
+        SizeOfV(prev) + WeightBucket(lastbucket);
+        //{ PkvMarshalling.SizeOfVWellMarshalledPackedKVIsBucketWeight(    FIXME
+        SizeOfV(v);
+      }
+    }
   }
 
   lemma SizeOfVTupleElem_le_SizeOfV(v: V, i: int)
